user 3, session 960, part 312

diffs-annotated-fixed/3/user-3-session-960.v
@@ -86,5 +86,74 @@ Class GoModel : Type :={byte : Type;
                         nilFile : File;
                         Ptr : Ptr.ty -> Type;
                         nullptr : forall ty, Ptr ty}.
+Opaque Nat.modulo Nat.div.
+#[local]Obligation Tactic := (intros; simpl; subst).
+Theorem mod_S_lt n m : n `mod` S m < S m.
+Proof.
+(apply PeanoNat.Nat.mod_upper_bound; auto).
+Qed.
+Function
+ nat_to_le base_m2 (x : nat) {wf lt x} : list {x : nat | x < S (S base_m2)}
+ :=
+   match x with
+   | 0 => nil
+   | _ =>
+       let base := S (S base_m2) in
+       let digit := x `mod` base in
+       exist (fun x => x < base) digit _ :: nat_to_le base_m2 (x / base)
+   end.
+Proof.
+-
+(intros; subst).
+(apply PeanoNat.Nat.div_lt; auto; try lia).
+-
+(apply lt_wf).
+Qed.
+Fixpoint le_to_nat base_m2 (digits : list {x : nat | x < S (S base_m2)}) :
+nat :=
+  match digits with
+  | nil => 0
+  | digit :: digits' => proj1_sig digit + le_to_nat digits' * S (S base_m2)
+  end.
+Redirect "/var/folders/5x/1mdbpbjd7012l971fq0zkj2w0000gn/T/coqlpFEfT"
+Print Ltac Signatures.
+Timeout 1 Print Grammar tactic.
+Add Search Blacklist "Raw" "Proofs".
+Set Search Output Name Only.
+Redirect "/var/folders/5x/1mdbpbjd7012l971fq0zkj2w0000gn/T/coqSBClfV"
+SearchPattern _.
+Remove Search Blacklist "Raw" "Proofs".
+Unset Search Output Name Only.
+Theorem nat_le_inverse base_m2 :
+  forall n, le_to_nat (nat_to_le base_m2 n) = n.
+Proof.
+(intros).
+(induction n as [n IHn] using lt_wf_ind).
+(destruct n; rewrite nat_to_le_equation; simpl).
+-
+auto.
+-
+(assert (1 < S (S base_m2)) by lia).
+(assert (base_m2 = S (S base_m2) - 2) by lia).
+(generalize dependent S (S base_m2); intros base **; subst).
+(assert (0 < S n) by lia).
+(generalize dependent S n; clear n; intros n **).
+(rewrite IHn).
+{
+(rewrite (PeanoNat.Nat.div_mod n base)  at 3 by lia).
+lia.
+}
+(apply Nat.div_lt; lia).
+Qed.
+Redirect "/var/folders/5x/1mdbpbjd7012l971fq0zkj2w0000gn/T/coqeJSuoV"
+Print Ltac Signatures.
+Timeout 1 Print Grammar tactic.
+Add Search Blacklist "Raw" "Proofs".
+Set Search Output Name Only.
+Redirect "/var/folders/5x/1mdbpbjd7012l971fq0zkj2w0000gn/T/coqFNw7z8"
+SearchPattern _.
+Remove Search Blacklist "Raw" "Proofs".
+Unset Search Output Name Only.
+Search -Ascii.ascii.
 (* Auto-generated comment: Succeeded. *)
 
